ovn/proofs/ssprove/extraction/Hacspec_ovn.v
@@ -22,9 +22,6 @@ From Hacspec Require Import Hacspec_Lib.
 Open Scope hacspec_scope.
 Import choice.Choice.Exports.
 
-Require Import ConCertLib.
-From ConCert.Execution Require Import Serializable.
-
 Obligation Tactic := (* try timeout 8 *) solve_ssprove_obligations.
 
 (*Not implemented yet? todo(item)*)
@@ -41,8 +38,8 @@ Class t_Group (Self : choice_type) := {
   t_group_type_t_Eq :> t_Eq (t_group_type) ;
   t_group_type_t_PartialEq :> t_PartialEq (t_group_type) ;
   t_group_type_t_Sized :> t_Sized (t_group_type) ;
-  q : forall {L1 I1}, both L1 I1 (int32) ;
-  g : forall {L1 I1}, both L1 I1 (t_group_type) ;
+  q : both (fset[]) (fset[]) (int32) ;
+  g : both (fset[]) (fset[]) (t_group_type) ;
   g_pow_loc : {fset Location} ;
   g_pow : forall {L1 I1}, both L1 I1 (int32) -> both (L1 :|: g_pow_loc) I1 (t_group_type) ;
   pow_loc : {fset Location} ;
@@ -72,24 +69,25 @@ Fail Next Obligation.
 
 Definition res_loc : Location :=
   (int32 ; 0%nat).
-
 #[global] Program Instance t_z_17__t_Group : t_Group t_z_17_ :=
   let t_group_type := int32 : choice_type in
-  let q := fun  {L : {fset Location}} {I : Interface} => solve_lift (ret_both (17 : int32)) : both L I (int32) in
-  let g := fun  {L : {fset Location}} {I : Interface} => solve_lift (ret_both (3 : int32)) : both L I (int32) in
-  let g_pow := fun  {L1 : {fset Location}} {I1 : Interface} (x : both L1 I1 (int32)) => solve_lift (((@g (fset []) (fset [])) .^ x) .% (@q (fset[]) (fset[]))) : both (L1 :|: fset []) I1 (int32) in
-  let pow := fun  {L1 : {fset Location}} {L2 : {fset Location}} {I1 : Interface} {I2 : Interface} (g : both L1 I1 (int32)) (x : both L2 I2 (int32)) => solve_lift ((g .^ x) .% (@q (fset[]) (fset[]))) : both (L1 :|: L2 :|: fset []) (I1 :|: I2) (int32) in
+  let q := ret_both (17 : int32) : both (fset []) (fset []) (int32) in
+  let g := ret_both (3 : int32) : both (fset []) (fset []) (int32) in
+  let g_pow := fun  {L1 : {fset Location}} {I1 : Interface} (x : both L1 I1 (int32)) => solve_lift ((g .^ x) .% q) : both (L1 :|: fset []) I1 (int32) in
+  let pow := fun  {L1 : {fset Location}} {L2 : {fset Location}} {I1 : Interface} {I2 : Interface} (g : both L1 I1 (int32)) (x : both L2 I2 (int32)) => solve_lift ((g .^ x) .% q) : both (L1 :|: L2 :|: fset []) (I1 :|: I2) (int32) in
   let one := fun  {L : {fset Location}} {I : Interface} => solve_lift (ret_both (1 : int32)) : both (L :|: fset []) I (int32) in
-  let prod := fun  {L1 : {fset Location}} {L2 : {fset Location}} {I1 : Interface} {I2 : Interface} (x : both L1 I1 (int32)) (y : both L2 I2 (int32)) => solve_lift ((x .* y) .% (@q (fset[]) (fset[]))) : both (L1 :|: L2 :|: fset []) (I1 :|: I2) (int32) in
+  let prod := fun  {L1 : {fset Location}} {L2 : {fset Location}} {I1 : Interface} {I2 : Interface} (x : both L1 I1 (int32)) (y : both L2 I2 (int32)) => solve_lift ((x .* y) .% q) : both (L1 :|: L2 :|: fset []) (I1 :|: I2) (int32) in
   let inv := fun  {L1 : {fset Location}} {I1 : Interface} (x : both L1 I1 (int32)) => letb res loc(res_loc) := ret_both (0 : int32) in
-  letb res := foldi_both (into_iter (Build_t_Range (f_start := ret_both (1 : int32)) (f_end := (@q (fset[]) (fset[]))))) (fun i =>
+  letb res := foldi_both_list (into_iter (Build_t_Range (f_start := ret_both (1 : int32)) (f_end := q))) (fun i =>
     ssp (fun res =>
+      letb i_computation := i in
       solve_lift (ifb (g_pow i) =.? x
-      then letb res := i in
+      then letb res := i_computation in
         res
-      else res))) res in
-  (* solve_lift *) res : both (L1 :|: fset [res_loc]) I1 (int32) in
-  let div := fun  {L1 : {fset Location}} {L2 : {fset Location}} {I1 : Interface} {I2 : Interface} (x : both L1 I1 (int32)) (y : both L2 I2 (int32)) => solve_lift (prod x (inv y)) : both (L1 :|: L2 :|: fset [res_loc]) (I1 :|: I2) (int32) in{| t_group_type := (@t_group_type);
+      else res) : both (*2*)(L1:|:fset [res_loc;res_loc]) (I1) (int32))) res in
+  solve_lift res : both (L1 :|: fset [res_loc]) I1 (int32) in
+  let div := fun  {L1 : {fset Location}} {L2 : {fset Location}} {I1 : Interface} {I2 : Interface} (x : both L1 I1 (int32)) (y : both L2 I2 (int32)) => solve_lift (prod x (inv y)) : both (L1 :|: L2 :|: fset [res_loc]) (I1 :|: I2) (int32) in
+  {| t_group_type := (@t_group_type);
   q := (@q);
   g := (@g);
   g_pow_loc := (fset [] : {fset Location});
@@ -103,9 +101,8 @@ Definition res_loc : Location :=
   inv_loc := (fset [res_loc] : {fset Location});
   inv := (@inv);
   div_loc := (fset [res_loc] : {fset Location});
-  div := (@div);
-  t_group_type_t_Eq := int_eqdec
-  |}.
+  div := (@div)|}.
+Solve All Obligations with exact int_eqdec.
 Fail Next Obligation.
 Hint Unfold t_z_17__t_Group.
 
@@ -164,14 +161,6 @@ Notation "'Build_t_OvnContractState' '[' x ']' '(' 'f_commit_vis' ':=' y ')'" :=
 Notation "'Build_t_OvnContractState' '[' x ']' '(' 'f_g_pow_xi_yi_vis' ':=' y ')'" := (Build_t_OvnContractState (f_g_pow_xis := f_g_pow_xis x) (f_zkp_xis := f_zkp_xis x) (f_commit_vis := f_commit_vis x) (f_g_pow_xi_yi_vis := y) (f_zkp_vis := f_zkp_vis x) (f_tally := f_tally x)).
 Notation "'Build_t_OvnContractState' '[' x ']' '(' 'f_zkp_vis' ':=' y ')'" := (Build_t_OvnContractState (f_g_pow_xis := f_g_pow_xis x) (f_zkp_xis := f_zkp_xis x) (f_commit_vis := f_commit_vis x) (f_g_pow_xi_yi_vis := f_g_pow_xi_yi_vis x) (f_zkp_vis := y) (f_tally := f_tally x)).
 Notation "'Build_t_OvnContractState' '[' x ']' '(' 'f_tally' ':=' y ')'" := (Build_t_OvnContractState (f_g_pow_xis := f_g_pow_xis x) (f_zkp_xis := f_zkp_xis x) (f_commit_vis := f_commit_vis x) (f_g_pow_xi_yi_vis := f_g_pow_xi_yi_vis x) (f_zkp_vis := f_zkp_vis x) (f_tally := y)).
-Definition state_OVN : choice_type :=
-  t_OvnContractState.
-Hint Unfold t_OvnContractState.
-Hint Unfold state_OVN.
-
-#[global] Program Instance serializable_state_OVN : Serializable state_OVN :=
-  ltac:(serialize_enum).
-Solve All Obligations with exact nseq_serializable || exact hacspec_int_serializable.
 
 Equations init_ovn_contract {L1 : {fset Location}} {I1 : Interface} {T : _} `{ t_Sized (T)} `{ t_HasInitContext (T) ('unit)} (ctx : both L1 I1 (T)) : both L1 I1 (t_Result (t_OvnContractState) (t_Reject)) :=
   init_ovn_contract ctx  :=
@@ -209,17 +198,25 @@ Fail Next Obligation.
 Notation "'Build_t_RegisterParam' '[' x ']' '(' 'f_rp_i' ':=' y ')'" := (Build_t_RegisterParam (f_rp_i := y) (f_rp_xi := f_rp_xi x)).
 Notation "'Build_t_RegisterParam' '[' x ']' '(' 'f_rp_xi' ':=' y ')'" := (Build_t_RegisterParam (f_rp_i := f_rp_i x) (f_rp_xi := y)).
 
-Equations register_vote {L1 : {fset Location}} {L2 : {fset Location}} {I1 : Interface} {I2 : Interface} {A : _} {T : _} `{ t_Sized (A)} `{ t_Sized (T)} `{ t_HasActions (A)} `{ t_HasReceiveContext (T) ('unit)} `{ t_Sized (A)} `{ t_Sized (T)} `{ t_HasActions (A)} `{ t_HasReceiveContext (T) ('unit)} (ctx : both L1 I1 (T)) (state : both L2 I2 (t_OvnContractState)) : both (L1 :|: L2) (I1 :|: I2) (t_Result ((A × t_OvnContractState)) (t_ParseError)) :=
+Definition register_vote_state_ret_loc {A : _} {T : _} `{ t_Sized (A)} `{ t_Sized (T)} `{ t_HasActions (A)} `{ t_HasReceiveContext (T) ('unit)} `{ t_Sized (A)} `{ t_Sized (T)} `{ t_HasActions (A)} `{ t_HasReceiveContext (T) ('unit)} : Location :=
+  (t_OvnContractState ; 1%nat).
+Equations register_vote {L1 : {fset Location}} {L2 : {fset Location}} {I1 : Interface} {I2 : Interface} {A : _} {T : _} `{ t_Sized (A)} `{ t_Sized (T)} `{ t_HasActions (A)} `{ t_HasReceiveContext (T) ('unit)} `{ t_Sized (A)} `{ t_Sized (T)} `{ t_HasActions (A)} `{ t_HasReceiveContext (T) ('unit)} (ctx : both L1 I1 (T)) (state : both L2 I2 (t_OvnContractState)) : both (L1 :|: L2 :|: fset [register_vote_state_ret_loc]) (I1 :|: I2) (t_Result ((A × t_OvnContractState)) (t_ParseError)) :=
   register_vote ctx state  :=
-    Result_Ok (solve_lift (prod_b (accept,state))) : both (L1 :|: L2) (I1 :|: I2) (t_Result ((A × t_OvnContractState)) (t_ParseError)).
+    solve_lift (run (letb '(_,out) := get (parameter_cursor ctx) in
+    letm[choice_typeMonad.result_bind_code (t_Result ((A × t_OvnContractState)) (t_ParseError))] (params:t_RegisterParam) := matchb branch out with
+    | ControlFlow_Break residual =>
+      letm[choice_typeMonad.result_bind_code (t_Result ((A × t_OvnContractState)) (t_ParseError))] hoist1 := v_Break (from_residual residual) in
+      ControlFlow_Continue (never_to_any hoist1)
+    | ControlFlow_Continue val =>
+      ControlFlow_Continue val
+    end in
+    ControlFlow_Continue (letb g_pow_xi := g_pow (f_rp_xi params) in
+    letb zkp_xi := v_ZKP g_pow_xi (f_rp_xi params) in
+    letb register_vote_state_ret loc(register_vote_state_ret_loc) := clone state in
+    letb register_vote_state_ret := Build_t_OvnContractState[register_vote_state_ret] (f_g_pow_xis := update_at (f_g_pow_xis register_vote_state_ret) (cast_int (WS2 := _) (f_rp_i params)) g_pow_xi) in
+    letb register_vote_state_ret := Build_t_OvnContractState[register_vote_state_ret] (f_zkp_xis := update_at (f_zkp_xis register_vote_state_ret) (cast_int (WS2 := _) (f_rp_i params)) zkp_xi) in
+    Result_Ok (prod_b (accept,register_vote_state_ret))))) : both (L1 :|: L2 :|: fset [register_vote_state_ret_loc]) (I1 :|: I2) (t_Result ((A × t_OvnContractState)) (t_ParseError)).
 Fail Next Obligation.
-Instance t_sized_register : t_Sized t_RegisterParam.
-Admitted.
-Instance t_has_receive_context_register : t_HasReceiveContext t_RegisterParam 'unit .
-Admitted.
-Equations receive_OVN_register {L1 L2 I1 I2} {A : _} `{ t_Sized (A)}`{ t_HasActions (A)} (ctx : both L1 I1 t_RegisterParam) (st : both L2 I2 (state_OVN)) : both (L1 :|: L2) (I1 :|: I2) (t_Result ((A × state_OVN)) (t_ParseError)) :=
-  receive_OVN_register ctx st :=
-  register_vote ctx st.
 
 Definition t_CastVoteParam : choice_type :=
   (int32 × int32 × 'bool).
@@ -254,24 +251,24 @@ Equations check_valid {L1 : {fset Location}} {I1 : Interface} (zkp : both L1 I1 
     solve_lift (ret_both (true : 'bool)) : both L1 I1 ('bool).
 Fail Next Obligation.
 
-Definition prod2_loc : Location :=
-  (int32 ; 2%nat).
 Definition prod1_loc : Location :=
-  (int32 ; 1%nat).
-Equations compute_group_element_for_vote {L1 : {fset Location}} {L2 : {fset Location}} {L3 : {fset Location}} {L4 : {fset Location}} {I1 : Interface} {I2 : Interface} {I3 : Interface} {I4 : Interface} (i : both L1 I1 (int32)) (xi : both L2 I2 (int32)) (vote : both L3 I3 ('bool)) (xis : both L4 I4 (nseq int32 20)) : both (L1 :|: L2 :|: L3 :|: L4 :|: fset [prod2_loc;prod1_loc;res_loc]) (I1 :|: I2 :|: I3 :|: I4) (int32) :=
+  (int32 ; 2%nat).
+Definition prod2_loc : Location :=
+  (int32 ; 3%nat).
+Equations compute_group_element_for_vote {L1 : {fset Location}} {L2 : {fset Location}} {L3 : {fset Location}} {L4 : {fset Location}} {I1 : Interface} {I2 : Interface} {I3 : Interface} {I4 : Interface} (i : both L1 I1 (int32)) (xi : both L2 I2 (int32)) (vote : both L3 I3 ('bool)) (xis : both L4 I4 (nseq int32 20)) : both (L1 :|: L2 :|: L3 :|: L4 :|: fset [prod1_loc;prod2_loc;res_loc]) (I1 :|: I2 :|: I3 :|: I4) (int32) :=
   compute_group_element_for_vote i xi vote xis  :=
-    (letb prod1 loc(prod1_loc) := one in
-    letb prod1 := foldi_both (L := (L1 :|: L2 :|: L3 :|: L4 :|: fset [prod2_loc;prod1_loc;res_loc])) (I := I1 :|: I2 :|: I3 :|: I4) (into_iter (Build_t_Range (f_start := ret_both (0 : uint_size)) (f_end := cast_int (WS2 := U32) (i .- (ret_both (1 : int32)))))) (fun j =>
+    letb prod1 loc(prod1_loc) := one in
+    letb prod1 := foldi_both_list (into_iter (Build_t_Range (f_start := ret_both (0 : uint_size)) (f_end := cast_int (WS2 := _) (i .- (ret_both (1 : int32)))))) (fun j =>
       ssp (fun prod1 =>
-             solve_lift (prod prod1 (xis.a[j])))) prod1 in
+        solve_lift (prod prod1 (xis.a[j])) : both (*2*)(L1:|:L4:|:L1:|:fset [prod1_loc;prod1_loc]) (I1:|:I4:|:I1) (t_group_type))) prod1 in
     letb prod2 loc(prod2_loc) := one in
-    letb prod2 := foldi_both (L := (L1 :|: L2 :|: L3 :|: L4 :|: fset [prod2_loc;prod1_loc;res_loc])) (I := I1 :|: I2 :|: I3 :|: I4) (into_iter (Build_t_Range (f_start := cast_int (WS2 := U32) (i .+ (ret_both (1 : int32)))) (f_end := n))) (fun j =>
+    letb prod2 := foldi_both_list (into_iter (Build_t_Range (f_start := cast_int (WS2 := _) (i .+ (ret_both (1 : int32)))) (f_end := n))) (fun j =>
       ssp (fun prod2 =>
-        solve_lift (prod prod2 (xis.a[j])))) prod2 in
+        solve_lift (prod prod2 (xis.a[j])) : both (*2*)(L1:|:L4:|:L1:|:fset [prod2_loc;prod2_loc]) (I1:|:I4:|:I1) (t_group_type))) prod2 in
     letb Yi := div prod1 prod2 in
     solve_lift (prod (pow Yi xi) (g_pow (ifb vote
     then ret_both (1 : int32)
-                                         else ret_both (0 : int32)))) : both (L1 :|: L2 :|: L3 :|: L4 :|: fset [prod2_loc;prod1_loc;res_loc]) (I1 :|: I2 :|: I3 :|: I4) (int32)).
+    else ret_both (0 : int32)))) : both (L1 :|: L2 :|: L3 :|: L4 :|: fset [prod1_loc;prod2_loc;res_loc]) (I1 :|: I2 :|: I3 :|: I4) (int32).
 Fail Next Obligation.
 
 Equations commit_to {L1 : {fset Location}} {I1 : Interface} (x : both L1 I1 (int32)) : both L1 I1 (int32) :=
@@ -279,29 +276,53 @@ Equations commit_to {L1 : {fset Location}} {I1 : Interface} (x : both L1 I1 (int
     solve_lift (ret_both (0 : int32)) : both L1 I1 (int32).
 Fail Next Obligation.
 
-Equations commit_to_vote {L1 : {fset Location}} {L2 : {fset Location}} {I1 : Interface} {I2 : Interface} {A : _} {(* impl *) HasReceiveContext : _} `{ t_Sized (A)} `{ t_Sized ((* impl *) HasReceiveContext)} `{ t_HasActions (A)} `{ t_HasReceiveContext (impl HasReceiveContext) ('unit)} `{ t_Sized (A)} `{ t_Sized (impl HasReceiveContext)} `{ t_HasActions (A)} `{ t_HasReceiveContext (impl HasReceiveContext) ('unit)} (ctx : both L1 I1 (impl HasReceiveContext)) (state : both L2 I2 (t_OvnContractState)) : both (L1 :|: L2) (I1 :|: I2) (t_Result ((A × t_OvnContractState)) (t_ParseError)) :=
+Definition commit_to_vote_state_ret_loc {A : _} {(* impl *) HasReceiveContext : _} `{ t_Sized (A)} `{ t_Sized ((* impl *) HasReceiveContext)} `{ t_HasActions (A)} `{ t_HasReceiveContext ((* impl *) HasReceiveContext) ('unit)} `{ t_Sized (A)} `{ t_Sized ((* impl *) HasReceiveContext)} `{ t_HasActions (A)} `{ t_HasReceiveContext ((* impl *) HasReceiveContext) ('unit)} : Location :=
+  (t_OvnContractState ; 4%nat).
+Equations commit_to_vote {L1 : {fset Location}} {L2 : {fset Location}} {I1 : Interface} {I2 : Interface} {A : _} {(* impl *) HasReceiveContext : _} `{ t_Sized (A)} `{ t_Sized ((* impl *) HasReceiveContext)} `{ t_HasActions (A)} `{ t_HasReceiveContext ((* impl *) HasReceiveContext) ('unit)} `{ t_Sized (A)} `{ t_Sized ((* impl *) HasReceiveContext)} `{ t_HasActions (A)} `{ t_HasReceiveContext ((* impl *) HasReceiveContext) ('unit)} (ctx : both L1 I1 ((* impl *) HasReceiveContext)) (state : both L2 I2 (t_OvnContractState)) : both (L1 :|: L2 :|: fset [commit_to_vote_state_ret_loc;prod1_loc;prod2_loc;res_loc]) (I1 :|: I2) (t_Result ((A × t_OvnContractState)) (t_ParseError)) :=
   commit_to_vote ctx state  :=
-    Result_Ok (solve_lift (prod_b (accept,state))) : both (L1 :|: L2) (I1 :|: I2) (t_Result ((A × t_OvnContractState)) (t_ParseError)).
+    solve_lift (run (letb '(_,out) := get (parameter_cursor ctx) in
+    letm[choice_typeMonad.result_bind_code (t_Result ((A × t_OvnContractState)) (t_ParseError))] (params:t_CastVoteParam) := matchb branch out with
+    | ControlFlow_Break residual =>
+      letm[choice_typeMonad.result_bind_code (t_Result ((A × t_OvnContractState)) (t_ParseError))] hoist2 := v_Break (from_residual residual) in
+      ControlFlow_Continue (never_to_any hoist2)
+    | ControlFlow_Continue val =>
+      ControlFlow_Continue val
+    end in
+    ControlFlow_Continue (letb _ := foldi_both_list (into_iter (f_zkp_xis state)) (fun zkp =>
+      ssp (fun _ =>
+        letb _ := check_valid zkp in
+        solve_lift (ret_both (tt : 'unit)) : both (*0*)(L2:|:fset []) (I2) ('unit))) (ret_both (tt : 'unit)) in
+    letb g_pow_xi_yi_vi := compute_group_element_for_vote (f_cvp_i params) (f_cvp_xi params) (f_cvp_vote params) (f_g_pow_xis state) in
+    letb commit_vi := commit_to g_pow_xi_yi_vi in
+    letb commit_to_vote_state_ret loc(commit_to_vote_state_ret_loc) := clone state in
+    letb commit_to_vote_state_ret := Build_t_OvnContractState[commit_to_vote_state_ret] (f_commit_vis := update_at (f_commit_vis commit_to_vote_state_ret) (cast_int (WS2 := _) (f_cvp_i params)) commit_vi) in
+    Result_Ok (prod_b (accept,commit_to_vote_state_ret))))) : both (L1 :|: L2 :|: fset [commit_to_vote_state_ret_loc;prod1_loc;prod2_loc;res_loc]) (I1 :|: I2) (t_Result ((A × t_OvnContractState)) (t_ParseError)).
 Fail Next Obligation.
-Instance t_sized_cast_vote_param : t_Sized t_CastVoteParam.
-Admitted.
-Instance t_has_receive_cast_vote_param : t_HasReceiveContext t_CastVoteParam 'unit .
-Admitted.
-Definition receive_OVN_commit_to_vote {L1 L2 I1 I2} {A : _} `{ t_Sized (A)}`{ t_HasActions (A)} (ctx : both L1 I1 t_CastVoteParam) (st : both L2 I2 (state_OVN)) : both (L1 :|: L2) (I1 :|: I2) (t_Result ((A × state_OVN)) (t_ParseError)) :=
-  commit_to_vote ctx st.
 
 Equations v_ZKP_one_out_of_two {L1 : {fset Location}} {L2 : {fset Location}} {I1 : Interface} {I2 : Interface} (g_pow_vi : both L1 I1 (int32)) (vi : both L2 I2 ('bool)) : both (L1 :|: L2) (I1 :|: I2) (int32) :=
   v_ZKP_one_out_of_two g_pow_vi vi  :=
     solve_lift (ret_both (32 : int32)) : both (L1 :|: L2) (I1 :|: I2) (int32).
 Fail Next Obligation.
 
-Equations cast_vote {L1 : {fset Location}} {L2 : {fset Location}} {I1 : Interface} {I2 : Interface} {A : _} {(* impl *) HasReceiveContext : _} `{ t_Sized (A)} `{ t_Sized ((* impl *) HasReceiveContext)} `{ t_HasActions (A)} `{ t_HasReceiveContext (impl HasReceiveContext) ('unit)} `{ t_Sized (A)} `{ t_Sized (impl HasReceiveContext)} `{ t_HasActions (A)} `{ t_HasReceiveContext (impl HasReceiveContext) ('unit)} (ctx : both L1 I1 (impl HasReceiveContext)) (state : both L2 I2 (t_OvnContractState)) : both (L1 :|: L2) (I1 :|: I2) (t_Result ((A × t_OvnContractState)) (t_ParseError)) :=
+Definition cast_vote_state_ret_loc {A : _} {(* impl *) HasReceiveContext : _} `{ t_Sized (A)} `{ t_Sized ((* impl *) HasReceiveContext)} `{ t_HasActions (A)} `{ t_HasReceiveContext ((* impl *) HasReceiveContext) ('unit)} `{ t_Sized (A)} `{ t_Sized ((* impl *) HasReceiveContext)} `{ t_HasActions (A)} `{ t_HasReceiveContext ((* impl *) HasReceiveContext) ('unit)} : Location :=
+  (t_OvnContractState ; 5%nat).
+Equations cast_vote {L1 : {fset Location}} {L2 : {fset Location}} {I1 : Interface} {I2 : Interface} {A : _} {(* impl *) HasReceiveContext : _} `{ t_Sized (A)} `{ t_Sized ((* impl *) HasReceiveContext)} `{ t_HasActions (A)} `{ t_HasReceiveContext ((* impl *) HasReceiveContext) ('unit)} `{ t_Sized (A)} `{ t_Sized ((* impl *) HasReceiveContext)} `{ t_HasActions (A)} `{ t_HasReceiveContext ((* impl *) HasReceiveContext) ('unit)} (ctx : both L1 I1 ((* impl *) HasReceiveContext)) (state : both L2 I2 (t_OvnContractState)) : both (L1 :|: L2 :|: fset [cast_vote_state_ret_loc;prod1_loc;prod2_loc;res_loc]) (I1 :|: I2) (t_Result ((A × t_OvnContractState)) (t_ParseError)) :=
   cast_vote ctx state  :=
-    Result_Ok (solve_lift (prod_b (accept,state))) : both (L1 :|: L2) (I1 :|: I2) (t_Result ((A × t_OvnContractState)) (t_ParseError)).
+    solve_lift (run (letb '(_,out) := get (parameter_cursor ctx) in
+    letm[choice_typeMonad.result_bind_code (t_Result ((A × t_OvnContractState)) (t_ParseError))] (params:t_CastVoteParam) := matchb branch out with
+    | ControlFlow_Break residual =>
+      letm[choice_typeMonad.result_bind_code (t_Result ((A × t_OvnContractState)) (t_ParseError))] hoist3 := v_Break (from_residual residual) in
+      ControlFlow_Continue (never_to_any hoist3)
+    | ControlFlow_Continue val =>
+      ControlFlow_Continue val
+    end in
+    ControlFlow_Continue (letb g_pow_xi_yi_vi := compute_group_element_for_vote (f_cvp_i params) (f_cvp_xi params) (f_cvp_vote params) (f_g_pow_xis state) in
+    letb zkp_vi := v_ZKP_one_out_of_two g_pow_xi_yi_vi (f_cvp_vote params) in
+    letb cast_vote_state_ret loc(cast_vote_state_ret_loc) := clone state in
+    letb cast_vote_state_ret := Build_t_OvnContractState[cast_vote_state_ret] (f_g_pow_xi_yi_vis := update_at (f_g_pow_xi_yi_vis cast_vote_state_ret) (cast_int (WS2 := _) (f_cvp_i params)) g_pow_xi_yi_vi) in
+    letb cast_vote_state_ret := Build_t_OvnContractState[cast_vote_state_ret] (f_zkp_vis := update_at (f_zkp_vis cast_vote_state_ret) (cast_int (WS2 := _) (f_cvp_i params)) zkp_vi) in
+    Result_Ok (prod_b (accept,cast_vote_state_ret))))) : both (L1 :|: L2 :|: fset [cast_vote_state_ret_loc;prod1_loc;prod2_loc;res_loc]) (I1 :|: I2) (t_Result ((A × t_OvnContractState)) (t_ParseError)).
 Fail Next Obligation.
-
-Definition receive_OVN_cast_vote {L1 L2 I1 I2} {A : _} `{ t_Sized (A)}`{ t_HasActions (A)} (ctx : both L1 I1 t_CastVoteParam) (st : both L2 I2 (state_OVN)) : both (L1 :|: L2) (I1 :|: I2) (t_Result ((A × state_OVN)) (t_ParseError)) :=
-  cast_vote ctx st.
 
 Equations check_valid2 {L1 : {fset Location}} {L2 : {fset Location}} {I1 : Interface} {I2 : Interface} (g_pow_xi_yi_vi : both L1 I1 (int32)) (zkp : both L2 I2 (int32)) : both (L1 :|: L2) (I1 :|: I2) ('bool) :=
   check_valid2 g_pow_xi_yi_vi zkp  :=
@@ -320,98 +341,115 @@ Equations Build_t_TallyParameter : both (fset []) (fset []) (t_TallyParameter) :
     solve_lift (ret_both ((_) : (t_TallyParameter))) : both (fset []) (fset []) (t_TallyParameter).
 Fail Next Obligation.
 
-Equations tally_votes {L1 : {fset Location}} {L2 : {fset Location}} {I1 : Interface} {I2 : Interface} {A : _} {(* impl *) HasReceiveContext : _} `{ t_Sized (A)} `{ t_Sized ((* impl *) HasReceiveContext)} `{ t_HasActions (A)} `{ t_HasReceiveContext (impl HasReceiveContext) ('unit)} `{ t_Sized (A)} `{ t_Sized (impl HasReceiveContext)} `{ t_HasActions (A)} `{ t_HasReceiveContext (impl HasReceiveContext) ('unit)} (_ : both L1 I1 (impl HasReceiveContext)) (state : both L2 I2 (t_OvnContractState)) : both (L1 :|: L2) (I1 :|: I2) (t_Result ((A × t_OvnContractState)) (t_ParseError)) :=
+Definition tally_loc {A : _} {(* impl *) HasReceiveContext : _} `{ t_Sized (A)} `{ t_Sized ((* impl *) HasReceiveContext)} `{ t_HasActions (A)} `{ t_HasReceiveContext ((* impl *) HasReceiveContext) ('unit)} `{ t_Sized (A)} `{ t_Sized ((* impl *) HasReceiveContext)} `{ t_HasActions (A)} `{ t_HasReceiveContext ((* impl *) HasReceiveContext) ('unit)} : Location :=
+  (int32 ; 6%nat).
+Definition tally_votes_state_ret_loc {A : _} {(* impl *) HasReceiveContext : _} `{ t_Sized (A)} `{ t_Sized ((* impl *) HasReceiveContext)} `{ t_HasActions (A)} `{ t_HasReceiveContext ((* impl *) HasReceiveContext) ('unit)} `{ t_Sized (A)} `{ t_Sized ((* impl *) HasReceiveContext)} `{ t_HasActions (A)} `{ t_HasReceiveContext ((* impl *) HasReceiveContext) ('unit)} : Location :=
+  (t_OvnContractState ; 7%nat).
+Definition vote_result_loc {A : _} {(* impl *) HasReceiveContext : _} `{ t_Sized (A)} `{ t_Sized ((* impl *) HasReceiveContext)} `{ t_HasActions (A)} `{ t_HasReceiveContext ((* impl *) HasReceiveContext) ('unit)} `{ t_Sized (A)} `{ t_Sized ((* impl *) HasReceiveContext)} `{ t_HasActions (A)} `{ t_HasReceiveContext ((* impl *) HasReceiveContext) ('unit)} : Location :=
+  (t_group_type ; 8%nat).
+Equations tally_votes {L1 : {fset Location}} {L2 : {fset Location}} {I1 : Interface} {I2 : Interface} {A : _} {(* impl *) HasReceiveContext : _} `{ t_Sized (A)} `{ t_Sized ((* impl *) HasReceiveContext)} `{ t_HasActions (A)} `{ t_HasReceiveContext ((* impl *) HasReceiveContext) ('unit)} `{ t_Sized (A)} `{ t_Sized ((* impl *) HasReceiveContext)} `{ t_HasActions (A)} `{ t_HasReceiveContext ((* impl *) HasReceiveContext) ('unit)} (_ : both L1 I1 ((* impl *) HasReceiveContext)) (state : both L2 I2 (t_OvnContractState)) : both (L1 :|: L2 :|: fset [tally_loc;tally_votes_state_ret_loc;vote_result_loc]) (I1 :|: I2) (t_Result ((A × t_OvnContractState)) (t_ParseError)) :=
   tally_votes _ state  :=
-    Result_Ok (solve_lift (prod_b (accept,state))) : both (L1 :|: L2) (I1 :|: I2) (t_Result ((A × t_OvnContractState)) (t_ParseError)).
+    letb _ := foldi_both_list (into_iter (Build_t_Range (f_start := ret_both (0 : uint_size)) (f_end := n))) (fun i =>
+      ssp (fun _ =>
+        letb _ := check_valid2 ((f_g_pow_xi_yi_vis state).a[i]) ((f_zkp_vis state).a[i]) in
+        letb _ := check_commitment ((f_g_pow_xi_yi_vis state).a[i]) ((f_commit_vis state).a[i]) in
+        solve_lift (ret_both (tt : 'unit)) : both (*0*)(L2:|:fset []) (I2) ('unit))) (ret_both (tt : 'unit)) in
+    letb (vote_result) loc(vote_result_loc) := one in
+    letb vote_result := foldi_both_list (into_iter (f_g_pow_xi_yi_vis state)) (fun g_pow_vote =>
+      ssp (fun vote_result =>
+        solve_lift (prod vote_result g_pow_vote) : both (*2*)(L2:|:L2:|:fset [vote_result_loc;vote_result_loc]) (I2:|:I2) (t_group_type))) vote_result in
+    letb tally loc(tally_loc) := ret_both (0 : int32) in
+    letb tally := foldi_both_list (into_iter (Build_t_Range (f_start := ret_both (0 : int32)) (f_end := cast_int (WS2 := _) n))) (fun i =>
+      ssp (fun tally =>
+        solve_lift (ifb (g_pow i) =.? vote_result
+        then letb tally := i in
+          tally
+        else tally) : both (*3*)(L2 :|: fset [tally_loc;vote_result_loc;tally_loc]) ((I2 :|: fset [])) (int32))) tally in
+    letb tally_votes_state_ret loc(tally_votes_state_ret_loc) := clone state in
+    letb tally_votes_state_ret := Build_t_OvnContractState[tally_votes_state_ret] (f_tally := tally) in
+    Result_Ok (solve_lift (prod_b (accept,tally_votes_state_ret))) : both (L1 :|: L2 :|: fset [tally_loc;tally_votes_state_ret_loc;vote_result_loc]) (I1 :|: I2) (t_Result ((A × t_OvnContractState)) (t_ParseError)).
 Fail Next Obligation.
 
-Instance t_sized_TallyParameter : t_Sized t_TallyParameter.
-Admitted.
-Instance t_has_receive_context_TallyParameter : t_HasReceiveContext t_TallyParameter 'unit .
-Admitted. 
-Definition receive_OVN_tally {L1 L2 I1 I2} {A : _} `{ t_Sized (A)}`{ t_HasActions (A)} (ctx : both L1 I1 t_TallyParameter) (st : both L2 I2 (state_OVN)) : both (L1 :|: L2) (I1 :|: I2) (t_Result ((A × state_OVN)) (t_ParseError)) :=
+(** Concert lib part **)
+From ConCert.Utils Require Import Extras.
+Export Extras.
+From ConCert.Utils Require Import Automation.
+Export Automation.
+From ConCert.Execution Require Import Serializable.
+Export Serializable.
+From ConCert.Execution Require Import Blockchain.
+Export Blockchain.
+From ConCert.Execution Require Import ContractCommon.
+Export ContractCommon.
+From ConCert.Execution Require Import Serializable.
+Export Serializable.
+Require Import ConCertLib.
+Export ConCertLib.
+
+Definition state_OVN : choice_type :=
+  t_OvnContractState.
+
+Definition init_OVN (chain : Chain) (ctx : ContractCallContext) (st : (state_OVN)) : ResultMonad.result ((state_OVN)) (t_ParseError) :=
+  ResultMonad.Ok st.
+
+#[global] Instance t_RegisterParam_t_HasReceiveContext : t_HasReceiveContext t_RegisterParam 'unit. Admitted.
+#[global] Instance t_RegisterParam_t_Sized : t_Sized t_RegisterParam. Admitted.
+Definition receive_OVN_register {A : _} {T : _} `{ t_Sized (A)} `{ t_Sized (T)} `{ t_HasActions (A)} `{ t_HasReceiveContext (T) ('unit)} `{ t_Sized (A)} `{ t_Sized (T)} `{ t_HasActions (A)} `{ t_HasReceiveContext (T) ('unit)} {L0 : {fset Location}} {L1 : {fset Location}} {I0 : Interface} {I1 : Interface} (ctx : both L0 I0 (t_RegisterParam)) (st : both L1 I1 (state_OVN)) : both _ _ (t_Result ((A × state_OVN)) (t_ParseError)) :=
+  register_vote ctx st.
+
+#[global] Instance t_CastVoteParam_t_HasReceiveContext : t_HasReceiveContext t_CastVoteParam 'unit. Admitted.
+#[global] Instance t_CastVoteParam_t_Sized : t_Sized t_CastVoteParam. Admitted.
+Definition receive_OVN_commit_to_vote {A : _} {(* impl *) HasReceiveContext : _} `{ t_Sized (A)} `{ t_Sized ((* impl *) HasReceiveContext)} `{ t_HasActions (A)} `{ t_HasReceiveContext ((* impl *) HasReceiveContext) ('unit)} `{ t_Sized (A)} `{ t_Sized ((* impl *) HasReceiveContext)} `{ t_HasActions (A)} `{ t_HasReceiveContext ((* impl *) HasReceiveContext) ('unit)} {L0 : {fset Location}} {L1 : {fset Location}} {I0 : Interface} {I1 : Interface} (ctx : both L0 I0 (t_CastVoteParam)) (st : both L1 I1 (state_OVN)) : both _ _ (t_Result ((A × state_OVN)) (t_ParseError)) :=
+  commit_to_vote ctx st.
+
+(* #[global] Instance t_CastVoteParam_t_HasReceiveContext : t_HasReceiveContext t_CastVoteParam 'unit. Admitted. *)
+(* #[global] Instance t_CastVoteParam_t_Sized : t_Sized t_CastVoteParam. Admitted. *)
+Definition receive_OVN_cast_vote {A : _} {(* impl *) HasReceiveContext : _} `{ t_Sized (A)} `{ t_Sized ((* impl *) HasReceiveContext)} `{ t_HasActions (A)} `{ t_HasReceiveContext ((* impl *) HasReceiveContext) ('unit)} `{ t_Sized (A)} `{ t_Sized ((* impl *) HasReceiveContext)} `{ t_HasActions (A)} `{ t_HasReceiveContext ((* impl *) HasReceiveContext) ('unit)} {L0 : {fset Location}} {L1 : {fset Location}} {I0 : Interface} {I1 : Interface} (ctx : both L0 I0 (t_CastVoteParam)) (st : both L1 I1 (state_OVN)) : both _ _ (t_Result ((A × state_OVN)) (t_ParseError)) :=
+  cast_vote ctx st.
+
+#[global] Instance t_TallyParameter_t_HasReceiveContext : t_HasReceiveContext t_TallyParameter 'unit. Admitted.
+#[global] Instance t_TallyParameter_t_Sized : t_Sized t_TallyParameter. Admitted.
+Definition receive_OVN_tally {A : _} {(* impl *) HasReceiveContext : _} `{ t_Sized (A)} `{ t_Sized ((* impl *) HasReceiveContext)} `{ t_HasActions (A)} `{ t_HasReceiveContext ((* impl *) HasReceiveContext) ('unit)} `{ t_Sized (A)} `{ t_Sized ((* impl *) HasReceiveContext)} `{ t_HasActions (A)} `{ t_HasReceiveContext ((* impl *) HasReceiveContext) ('unit)} {L0 : {fset Location}} {L1 : {fset Location}} {I0 : Interface} {I1 : Interface} (ctx : both L0 I0 (t_TallyParameter)) (st : both L1 I1 (state_OVN)) : both _ _ (t_Result ((A × state_OVN)) (t_ParseError)) :=
   tally_votes ctx st.
 
-From ConCert.Execution Require Import Blockchain.
+Obligation Tactic := (* try timeout 8 *) solve_ssprove_obligations.
 
-Instance BaseTypes : ConCert.Execution.Blockchain.ChainBase :=
-  {|
-    Address := nat;
-    address_eqb := Nat.eqb ;
-    address_eqb_spec := Nat.eqb_spec;
-    address_is_contract := Nat.even;
-  |}.
-
-Instance t_sized_state_OVN : t_Sized state_OVN.
-Admitted.
-
-Instance t_HasActions_state_OVN : t_HasActions state_OVN.
-Admitted.
-
-
-Definition init_OVN {L : {fset Location}} {I : Interface} (chain : Chain) (ctx : ContractCallContext) (st : both L I (state_OVN)) : ResultMonad.result (both L I (state_OVN)) (t_ParseError) :=
-  ResultMonad.Ok st.
 Inductive Msg_OVN: Type :=
 | msg_OVN_register : t_RegisterParam -> Msg_OVN
 | msg_OVN_commit_to_vote : t_CastVoteParam -> Msg_OVN
 | msg_OVN_cast_vote : t_CastVoteParam -> Msg_OVN
 | msg_OVN_tally : t_TallyParameter -> Msg_OVN.
-Equations receive_OVN {L I} (chain : Chain) (ctx : ContractCallContext) (st : both L I (state_OVN)) (msg : Datatypes.option Msg_OVN) : ResultMonad.result (both L I state_OVN * list ActionBody) t_ParseError :=
-  receive_OVN chain ctx st msg :=
-  match msg with
-  | Some (msg_OVN_register val) =>
-      match (is_pure (both_prog (receive_OVN_register (ret_both val) (st)))) with
-         | inl x => ResultMonad.Ok (solve_lift ret_both (fst x), [])
+#[global] Instance state_OVN_t_HasReceiveContext : t_HasReceiveContext state_OVN 'unit. Admitted.
+#[global] Instance state_OVN_t_Sized : t_Sized state_OVN. Admitted.
+#[global] Instance state_OVN_t_HasActions : t_HasActions state_OVN. Admitted.
+Equations receive_OVN (chain : Chain) (ctx : ContractCallContext) (st : (state_OVN)) (msg : Datatypes.option Msg_OVN) : ResultMonad.result (state_OVN * list ActionBody) t_ParseError :=
+  receive_OVN chain ctx st msg  :=
+    match msg with
+    | Some (msg_OVN_register val) =>
+      match (is_pure (both_prog (receive_OVN_register (ret_both val) (ret_both st)))) with
+         | inl x => ResultMonad.Ok ((fst x), [])
          | inr x => ResultMonad.Err x
          end
-  | Some (msg_OVN_commit_to_vote val) =>
-    match (is_pure (both_prog (receive_OVN_commit_to_vote (ret_both val) (st)))) with
-         | inl x => ResultMonad.Ok (solve_lift ret_both (fst x), [])
+    | Some (msg_OVN_commit_to_vote val) =>
+      match (is_pure (both_prog (receive_OVN_commit_to_vote (ret_both val) (ret_both st)))) with
+         | inl x => ResultMonad.Ok ((fst x), [])
          | inr x => ResultMonad.Err x
          end
-  | Some (msg_OVN_cast_vote val) =>
-    match (is_pure (both_prog (receive_OVN_cast_vote (ret_both val) (st)))) with
-         | inl x => ResultMonad.Ok (solve_lift ret_both (fst x), [])
+    | Some (msg_OVN_cast_vote val) =>
+      match (is_pure (both_prog (receive_OVN_cast_vote (ret_both val) (ret_both st)))) with
+         | inl x => ResultMonad.Ok ((fst x), [])
          | inr x => ResultMonad.Err x
          end
-  | Some (msg_OVN_tally val) =>
-    match (is_pure (both_prog (receive_OVN_tally (ret_both val) (st)))) with
-         | inl x => ResultMonad.Ok (solve_lift ret_both (fst x), [])
+    | Some (msg_OVN_tally val) =>
+      match (is_pure (both_prog (receive_OVN_tally (ret_both val) (ret_both st)))) with
+         | inl x => ResultMonad.Ok ((fst x), [])
          | inr x => ResultMonad.Err x
          end
-  | _ =>
-    ResultMonad.Err tt
-  end.
+    | _ =>
+      ResultMonad.Err tt
+    end : ResultMonad.result (state_OVN * list ActionBody) t_ParseError.
 Fail Next Obligation.
-
-Inductive temp: Type :=
-| temp_OVN : temp.
-
-Instance serializable_both {L I} {A : choice_type} `{Serializable A} : Serializable (both L I A).
-Proof.
-Admitted.
-
-Instance serializable_Msg_OVN : Serializable Msg_OVN :=
-  (@serialize_by_other_option (Datatypes.option t_RegisterParam *
-                         Datatypes.option t_CastVoteParam *
-                         Datatypes.option t_CastVoteParam *
-                         Datatypes.option t_TallyParameter)
-                      _
-                      (fun m => match m with
-                             | @msg_OVN_register v => Some (Some v, None, None, None)
-                             | @msg_OVN_commit_to_vote v => Some (None, Some v, None, None)
-                             | @msg_OVN_cast_vote v => Some (None, None, Some v, None)
-                             | @msg_OVN_tally v => Some (None, None, None, Some v)
-                             end
-                      )
-                      (fun m => match m with
-                             | Some (Some v, _, _, _) => Some (msg_OVN_register v)
-                             | Some (_, Some v, _, _) => Some (msg_OVN_commit_to_vote v)
-                             | Some (_, _, Some v, _) => Some (msg_OVN_cast_vote v)
-                             | Some (_, _, _, Some v) => Some (msg_OVN_tally v)
-                             | _ => None
-                             end)
-                      (ltac:(destruct m ; reflexivity)) _).
-
-Definition contract_OVN {L I} : Contract (both L I state_OVN) (Msg_OVN) (both L I state_OVN) (t_ParseError) :=
+#[global] Instance state_OVN_Serializable : Serializable state_OVN. Admitted.
+#[global] Instance Msg_OVN_Serializable : Serializable Msg_OVN. Admitted.
+Definition contract_OVN : Contract ((state_OVN)) (Msg_OVN) ((state_OVN)) (t_ParseError) :=
   build_contract init_OVN receive_OVN.
